more work on getting the document into shape
Signed-off-by: Reto Achermann <achreto@gmail.com>

CleanQ/CleanQ_SetModel.thy
@@ -12,51 +12,64 @@
 
 
 
-section "CleanQ Abstract Set Model"
+section \<open>Abstract CleanQ Set Model\<close>
 
 text \<open>
-  We define
+  We define the CleanQ set model in the the following Isabelle theory: 
 \<close>
 
 theory CleanQ_SetModel
 (*<*)
   imports  "../Simpl/Vcg"
-(*>*)
 begin
+(*>*)
 
-
+text \<open>
+  We now define the model state, its invariants and state transitions. Followed by proofs 
+  using Owicki-Gries (OG)
+\<close>
 
 (* ==================================================================================== *)
-subsection \<open>State Definition\<close>
+subsection \<open>CleanQ Set Model State\<close>
 (* ==================================================================================== *)
 
+text \<open>
+  We model a system with a single point-to-point queue between two agents $X$ and $Y$.
+  The state of the abstract CleanQ Set model is captured in the Isabelle record
+  \verb+CleanQ_Set_State+. It consists of four sets, each of which capturing the ownership 
+  of buffer elements in the system. The sets can be divided into two groups: First, 
+  buffer elements that are owned by either $X$ or $Y$, and secondly, buffer elements that
+  are in transfer between $X$ and $Y$ or between $Y$ and $X$:
 
-subsubsection \<open>Abstract Queue Definition\<close>
+  \<^item> SX: this is the set of buffers owned by X.
+  \<^item> SY: this is the set of buffers owned by Y.
+  \<^item> TXY: this is the set of buffers in transfer from X to Y.
+  \<^item> TYX: this is the set of buffers in transfer from Y to X.
+\<close>
 
-text \<open>The "SetRB" defines the base state with four sets:
-  * SX: this is the set of buffers owned by X.
-  * SY: this is the set of buffers owned by Y.
-  * TXY: this is the set of buffers in transfer from X -> Y.
-  * TYX: this is the set of buffers in transfer from Y -> X.
-  
-  * Buffers in TXY and TYX are not owned by either X or Y.\<close>
-
-record 'a SetRB =
+record 'a CleanQ_Set_State =
   SX  :: "'a set"
   SY  :: "'a set"
   TXY :: "'a set"
   TYX :: "'a set"
 
+text \<open>
+  Note, we do not specify the representation of the buffer elements. This can be a single,
+  fixed-sized page frame, a variable-sized base-limit segment, or a set of memory 
+  locations. 
+\<close>
 
-record 'g SetRB_vars = 
-  RB_'  :: "nat SetRB"
+(*<*)
+(* Define some global variables to make Simpl/Complex proofs work *)
+record 'g CleanQ_Set_State_vars = 
+  RB_'  :: "nat CleanQ_Set_State"
   B_'   ::  nat
-
+(*>*)
   
 
 
 (* ==================================================================================== *)
-subsection \<open>State Invariants\<close>
+subsection \<open>CleanQ Set Model Invariants\<close>
 (* ==================================================================================== *)
 
 
@@ -69,7 +82,7 @@ text \<open>
   the ownership transfer
 \<close>
 
-fun I1 :: "'a SetRB \<Rightarrow> 'a set \<Rightarrow> bool"
+fun I1 :: "'a CleanQ_Set_State \<Rightarrow> 'a set \<Rightarrow> bool"
   where "I1 rb K \<longleftrightarrow> ((SX rb) \<union> (SY rb) \<union> (TXY rb) \<union> (TYX rb)) = K"
 
 
@@ -80,17 +93,17 @@ subsubsection \<open>I2: No Double Presence\<close>
 text \<open>All pairwise intersubsections are empty. An element cannot be in one than more sets. 
 This is required as the element cannot be owned by more than one agent.\<close>
 
-fun I2 :: "'a SetRB \<Rightarrow> bool"
+fun I2 :: "'a CleanQ_Set_State \<Rightarrow> bool"
   where "I2 rb \<longleftrightarrow> SX rb \<inter> SY rb = {} \<and> SX rb \<inter> TXY rb = {} \<and> SX rb \<inter> TYX rb = {} \<and> 
                    SY rb \<inter> TXY rb = {} \<and> SY rb \<inter> TYX rb = {} \<and> TXY rb \<inter> TYX rb = {}"
 
 
 (* ------------------------------------------------------------------------------------ *)
-subsubsection \<open>SetRB Invariants\<close>
+subsubsection \<open>Invariants\<close>
 (* ------------------------------------------------------------------------------------ *)
 
-fun SetRB_Invariants :: "'a set \<Rightarrow> 'a SetRB \<Rightarrow> bool"
-  where "SetRB_Invariants K rb \<longleftrightarrow> I1 rb K \<and> I2 rb"
+fun CleanQ_Set_State_Invariants :: "'a set \<Rightarrow> 'a CleanQ_Set_State \<Rightarrow> bool"
+  where "CleanQ_Set_State_Invariants K rb \<longleftrightarrow> I1 rb K \<and> I2 rb"
 
 
 (* ==================================================================================== *)
@@ -109,84 +122,84 @@ text \<open>
   TYX respectively.
 \<close>
 
-definition SetRB_enq_x :: "'a \<Rightarrow> 'a SetRB  \<Rightarrow> 'a SetRB"
-  where "SetRB_enq_x b rb = rb  \<lparr>  SX := (SX rb) - {(b)},  TXY := ((TXY rb) \<union> {(b)}) \<rparr>"
+definition CleanQ_Set_enq_x :: "'a \<Rightarrow> 'a CleanQ_Set_State  \<Rightarrow> 'a CleanQ_Set_State"
+  where "CleanQ_Set_enq_x b rb = rb  \<lparr>  SX := (SX rb) - {(b)},  TXY := ((TXY rb) \<union> {(b)}) \<rparr>"
 
-definition SetRB_enq_y :: "'a \<Rightarrow> 'a SetRB  \<Rightarrow> 'a SetRB"
-  where "SetRB_enq_y b rb = rb  \<lparr>  SY := (SY rb) - {(b)},  TYX := ((TYX rb) \<union> {(b)}) \<rparr>"
+definition CleanQ_Set_enq_y :: "'a \<Rightarrow> 'a CleanQ_Set_State  \<Rightarrow> 'a CleanQ_Set_State"
+  where "CleanQ_Set_enq_y b rb = rb  \<lparr>  SY := (SY rb) - {(b)},  TYX := ((TYX rb) \<union> {(b)}) \<rparr>"
 
 (*<*)
 
-lemma SetRB_enq_x_upd :
-  "SetRB_enq_x b rb =  \<lparr>  SX = (SX rb) - {(b)},  SY = (SY rb), TXY = ((TXY rb) \<union> {(b)}),  
+lemma CleanQ_Set_enq_x_upd :
+  "CleanQ_Set_enq_x b rb =  \<lparr>  SX = (SX rb) - {(b)},  SY = (SY rb), TXY = ((TXY rb) \<union> {(b)}),  
                           TYX = (TYX rb) \<rparr>"
-  by(simp add:SetRB_enq_x_def)
+  by(simp add:CleanQ_Set_enq_x_def)
 
-lemma SetRB_enq_y_upd :
-  "SetRB_enq_y b rb =  \<lparr>  SX = (SX rb),  SY = (SY rb) - {(b)}, TXY = (TXY rb),  
+lemma CleanQ_Set_enq_y_upd :
+  "CleanQ_Set_enq_y b rb =  \<lparr>  SX = (SX rb),  SY = (SY rb) - {(b)}, TXY = (TXY rb),  
                           TYX = ((TYX rb) \<union> {(b)}) \<rparr>"
-  by(simp add:SetRB_enq_y_def)
+  by(simp add:CleanQ_Set_enq_y_def)
 
 (*>*)
 
 
-text \<open>Next, we show that SetRB\_enqueuex preserves the invariant\<close>
+text \<open>Next, we show that CleanQ\_Set\_enqueuex preserves the invariant\<close>
 
-lemma SetRB_enq_x_I1 :
+lemma CleanQ_Set_enq_x_I1 :
   assumes I1_holds : "I1 rb K"
       and I2_holds : "I2 rb"
       and X_owned: "b \<in> SX rb"
-    shows "I1 (SetRB_enq_x b rb) K"
-  unfolding SetRB_enq_x_def 
+    shows "I1 (CleanQ_Set_enq_x b rb) K"
+  unfolding CleanQ_Set_enq_x_def 
   using I1_holds X_owned by auto
 
-lemma SetRB_enq_x_I2 :
+lemma CleanQ_Set_enq_x_I2 :
   assumes I1_holds : "I1 rb K"
       and I2_holds : "I2 rb"
       and X_owned: "b \<in> SX rb"
-    shows "I2 (SetRB_enq_x b rb)"
-  unfolding SetRB_enq_x_def
+    shows "I2 (CleanQ_Set_enq_x b rb)"
+  unfolding CleanQ_Set_enq_x_def
   using I2_holds X_owned by auto
 
-lemma SetRB_enq_x_Invariants :
-  assumes I_holds : "SetRB_Invariants K rb"
+lemma CleanQ_Set_enq_x_Invariants :
+  assumes I_holds : "CleanQ_Set_State_Invariants K rb"
       and X_owned: "b \<in> SX rb"
-    shows "SetRB_Invariants K (SetRB_enq_x b rb)"  
-  by (meson I_holds SetRB_Invariants.simps SetRB_enq_x_I1 SetRB_enq_x_I2 X_owned)
+    shows "CleanQ_Set_State_Invariants K (CleanQ_Set_enq_x b rb)"  
+  by (meson I_holds CleanQ_Set_State_Invariants.simps CleanQ_Set_enq_x_I1 CleanQ_Set_enq_x_I2 X_owned)
 
 
 
 
 
-lemma SetRB_Enq_Preserves_Invariants : 
-  "\<Gamma>\<turnstile> \<lbrace> rb' = \<acute>RB \<and> SetRB_Invariants K \<acute>RB \<and>  b \<in> SX \<acute>RB   \<rbrace> 
-        \<acute>RB :== (SetRB_enq_x b \<acute>RB) 
-      \<lbrace> SetRB_Invariants K \<acute>RB \<rbrace>"
+lemma CleanQ_Set_State_Enq_Preserves_Invariants : 
+  "\<Gamma>\<turnstile> \<lbrace> rb' = \<acute>RB \<and> CleanQ_Set_State_Invariants K \<acute>RB \<and>  b \<in> SX \<acute>RB   \<rbrace> 
+        \<acute>RB :== (CleanQ_Set_enq_x b \<acute>RB) 
+      \<lbrace> CleanQ_Set_State_Invariants K \<acute>RB \<rbrace>"
   apply vcg
-  by(simp only: SetRB_enq_x_Invariants)
+  by(simp only: CleanQ_Set_enq_x_Invariants)
 
 
-lemma SetRB_Enq_two_step:
-  "\<Gamma>\<turnstile> \<lbrace> rb' = \<acute>RB \<and> SetRB_Invariants K \<acute>RB \<and>  b \<in> SX \<acute>RB   \<rbrace>
+lemma CleanQ_Set_State_Enq_two_step:
+  "\<Gamma>\<turnstile> \<lbrace> rb' = \<acute>RB \<and> CleanQ_Set_State_Invariants K \<acute>RB \<and>  b \<in> SX \<acute>RB   \<rbrace>
             \<acute>RB :== \<acute>RB \<lparr>  SX := (SX  \<acute>RB ) - {(b)}  \<rparr> ;;
             \<acute>RB :==  \<acute>RB \<lparr>  TXY := ((TXY  \<acute>RB ) \<union> {(b)}) \<rparr>  
-      \<lbrace> \<acute>RB = SetRB_enq_x b rb' \<rbrace>"
+      \<lbrace> \<acute>RB = CleanQ_Set_enq_x b rb' \<rbrace>"
   apply vcg
-  by(simp add:SetRB_enq_x_def)
+  by(simp add:CleanQ_Set_enq_x_def)
 
 
-lemma "\<Gamma>\<turnstile> \<lbrace> rb' = \<acute>RB \<and> SetRB_Invariants K \<acute>RB \<and>  b \<in> SX \<acute>RB   \<rbrace>
+lemma "\<Gamma>\<turnstile> \<lbrace> rb' = \<acute>RB \<and> CleanQ_Set_State_Invariants K \<acute>RB \<and>  b \<in> SX \<acute>RB   \<rbrace>
            \<acute>RB :== \<acute>RB \<lparr>  SX := (SX rb) - {(b)}  \<rparr> ;;
            \<acute>RB :==  \<acute>RB \<lparr>  TXY := ((TXY rb) \<union> {(b)}) \<rparr>  
-            \<lbrace> SetRB_Invariants K \<acute>RB \<and> \<acute>RB = SetRB_enq_x b rb' \<rbrace>"
-  using  SetRB_Enq_two_step SetRB_Enq_Preserves_Invariants
+            \<lbrace> CleanQ_Set_State_Invariants K \<acute>RB \<and> \<acute>RB = CleanQ_Set_enq_x b rb' \<rbrace>"
+  using  CleanQ_Set_State_Enq_two_step CleanQ_Set_State_Enq_Preserves_Invariants
   oops
   
 
-lemma "\<Gamma>\<turnstile> \<lbrace> SetRB_Invariants K \<acute>RB  \<rbrace> 
-          IF b \<in> SX \<acute>RB THEN \<acute>RB :== (SetRB_enq_x b \<acute>RB) FI \<lbrace> SetRB_Invariants K \<acute>RB \<rbrace>"
+lemma "\<Gamma>\<turnstile> \<lbrace> CleanQ_Set_State_Invariants K \<acute>RB  \<rbrace> 
+          IF b \<in> SX \<acute>RB THEN \<acute>RB :== (CleanQ_Set_enq_x b \<acute>RB) FI \<lbrace> CleanQ_Set_State_Invariants K \<acute>RB \<rbrace>"
   apply vcg 
-  by (meson SetRB_enq_x_Invariants)
+  by (meson CleanQ_Set_enq_x_Invariants)
 
 
 
@@ -200,52 +213,52 @@ text \<open>
   corresponds to removing the element from set TYX and inserting it into set SX.
 \<close>
 
-definition SetRB_dequeuex :: "'a \<Rightarrow> 'a SetRB  \<Rightarrow> 'a SetRB"
-  where "SetRB_dequeuex b rb =  \<lparr>  SX = (SX rb) \<union> {(b)},  SY = (SY rb), TXY = (TXY rb),  
+definition CleanQ_Set_deq_x :: "'a \<Rightarrow> 'a CleanQ_Set_State  \<Rightarrow> 'a CleanQ_Set_State"
+  where "CleanQ_Set_deq_x b rb =  \<lparr>  SX = (SX rb) \<union> {(b)},  SY = (SY rb), TXY = (TXY rb),  
                                    TYX = (TYX rb) - {b} \<rparr>"
 
 
-text \<open>Next, we show that SetRB\_deuquex preserves the invariant\<close>
+text \<open>Next, we show that CleanQ\_Set\_deuquex preserves the invariant\<close>
 
-lemma SetRB_dequeuex_I1 :
+lemma CleanQ_Set_deq_x_I1 :
   assumes I1_holds : "I1 rb K"
       and I2_holds : "I2 rb"
       and TXY_owned: "b \<in> TXY rb"
-    shows "I1 (SetRB_dequeuex b rb) K"
-  unfolding SetRB_dequeuex_def
+    shows "I1 (CleanQ_Set_deq_x b rb) K"
+  unfolding CleanQ_Set_deq_x_def
   using I1_holds TXY_owned by auto
 
-lemma SetRB_dequeuex_I2 :
+lemma CleanQ_Set_deq_x_I2 :
   assumes I1_holds : "I1 rb K"
       and I2_holds : "I2 rb"
       and TYX_owned: "b \<in> TYX rb"
-    shows "I2 (SetRB_dequeuex b rb)"
-  unfolding SetRB_dequeuex_def
+    shows "I2 (CleanQ_Set_deq_x b rb)"
+  unfolding CleanQ_Set_deq_x_def
   using I2_holds TYX_owned by auto
 
-lemma SetRB_dequeuex_Invariants :
- assumes I_holds : "SetRB_Invariants K rb"
+lemma CleanQ_Set_deq_x_Invariants :
+ assumes I_holds : "CleanQ_Set_State_Invariants K rb"
       and TYX_owned: "b \<in> TYX rb"
-    shows "SetRB_Invariants K (SetRB_dequeuex b rb)" 
+    shows "CleanQ_Set_State_Invariants K (CleanQ_Set_deq_x b rb)" 
 proof -
   have "I1 \<lparr>SX = SX rb \<union> {b}, SY = SY rb, TXY = TXY rb, TYX = TYX rb - {b}\<rparr> K"
     using I_holds TYX_owned by auto
   then show ?thesis
-    by (metis I_holds SetRB_Invariants.simps SetRB_dequeuex_I2 SetRB_dequeuex_def TYX_owned)
+    by (metis I_holds CleanQ_Set_State_Invariants.simps CleanQ_Set_deq_x_I2 CleanQ_Set_deq_x_def TYX_owned)
 qed
 
 
 
 
-lemma "\<Gamma>\<turnstile> \<lbrace> SetRB_Invariants K \<acute>RB \<and>  b \<in> TYX \<acute>RB   \<rbrace> \<acute>RB :== (SetRB_dequeuex b \<acute>RB) \<lbrace> SetRB_Invariants K \<acute>RB \<rbrace>"
+lemma "\<Gamma>\<turnstile> \<lbrace> CleanQ_Set_State_Invariants K \<acute>RB \<and>  b \<in> TYX \<acute>RB   \<rbrace> \<acute>RB :== (CleanQ_Set_deq_x b \<acute>RB) \<lbrace> CleanQ_Set_State_Invariants K \<acute>RB \<rbrace>"
   apply vcg
-  by(simp only: SetRB_dequeuex_Invariants)
+  by(simp only: CleanQ_Set_deq_x_Invariants)
   
 
-lemma "\<Gamma>\<turnstile> \<lbrace> SetRB_Invariants K \<acute>RB  \<rbrace> 
-          IF b \<in> TYX \<acute>RB THEN \<acute>RB :== (SetRB_dequeuex b \<acute>RB) FI \<lbrace> SetRB_Invariants K \<acute>RB \<rbrace>"
+lemma "\<Gamma>\<turnstile> \<lbrace> CleanQ_Set_State_Invariants K \<acute>RB  \<rbrace> 
+          IF b \<in> TYX \<acute>RB THEN \<acute>RB :== (CleanQ_Set_deq_x b \<acute>RB) FI \<lbrace> CleanQ_Set_State_Invariants K \<acute>RB \<rbrace>"
   apply vcg 
-  by (meson SetRB_dequeuex_Invariants)
+  by (meson CleanQ_Set_deq_x_Invariants)
 
 
 (* ==================================================================================== *)
@@ -257,11 +270,11 @@ subsection \<open>Basic Integration\<close>
 subsubsection \<open>Enqueue Operation\<close>
 (* ------------------------------------------------------------------------------------ *)
 
-definition SetRB_enqueuex_pre :: "'a set \<Rightarrow> 'a \<Rightarrow> ('a SetRB, 'a SetRB) Semantic.xstate set"
-  where "SetRB_enqueuex_pre K b = Semantic.Normal ` { rb. I1 rb K \<and> I2 rb \<and> b \<in> SX rb }"
+definition CleanQ_Set_State_enqueuex_pre :: "'a set \<Rightarrow> 'a \<Rightarrow> ('a CleanQ_Set_State, 'a CleanQ_Set_State) Semantic.xstate set"
+  where "CleanQ_Set_State_enqueuex_pre K b = Semantic.Normal ` { rb. I1 rb K \<and> I2 rb \<and> b \<in> SX rb }"
 
-definition SetRB_enqueuex_post :: "'a set \<Rightarrow> 'a \<Rightarrow> ('a SetRB, 'a SetRB) Semantic.xstate set"
-  where "SetRB_enqueuex_post K b = Semantic.Normal ` { rb. I1 rb K \<and> I2 rb \<and> b \<in> TXY rb }"
+definition CleanQ_Set_State_enqueuex_post :: "'a set \<Rightarrow> 'a \<Rightarrow> ('a CleanQ_Set_State, 'a CleanQ_Set_State) Semantic.xstate set"
+  where "CleanQ_Set_State_enqueuex_post K b = Semantic.Normal ` { rb. I1 rb K \<and> I2 rb \<and> b \<in> TXY rb }"
 
 
 
@@ -270,11 +283,11 @@ subsubsection \<open>Dequeue Operation\<close>
 (* ------------------------------------------------------------------------------------ *)
 
 
-definition SetRB_dequeuex_pre :: "'a set \<Rightarrow> 'a \<Rightarrow> ('a SetRB, 'a SetRB) Semantic.xstate set"
-  where "SetRB_dequeuex_pre K b = Semantic.Normal ` { rb. I1 rb K \<and> I2 rb \<and> b \<in> TXY rb }"
+definition CleanQ_Set_deq_x_pre :: "'a set \<Rightarrow> 'a \<Rightarrow> ('a CleanQ_Set_State, 'a CleanQ_Set_State) Semantic.xstate set"
+  where "CleanQ_Set_deq_x_pre K b = Semantic.Normal ` { rb. I1 rb K \<and> I2 rb \<and> b \<in> TXY rb }"
 
-definition SetRB_dequeuex_post :: "'a set \<Rightarrow> 'a \<Rightarrow> ('a SetRB, 'a SetRB) Semantic.xstate set"
-  where "SetRB_dequeuex_post K b = Semantic.Normal ` { rb. I1 rb K \<and> I2 rb \<and> b \<in> SX rb }"
+definition CleanQ_Set_deq_x_post :: "'a set \<Rightarrow> 'a \<Rightarrow> ('a CleanQ_Set_State, 'a CleanQ_Set_State) Semantic.xstate set"
+  where "CleanQ_Set_deq_x_post K b = Semantic.Normal ` { rb. I1 rb K \<and> I2 rb \<and> b \<in> SX rb }"
 
 
 
